Superposition_Calculus/First_Order_Superposition_Soundness.thy
@@ -23,13 +23,13 @@ proof (cases P C rule: eq_resolution.cases)
     "\<And>I \<gamma> \<F>\<^sub>G. \<lbrakk>
         refl I; 
         \<forall>P\<^sub>G. (\<exists>\<gamma>'. P\<^sub>G = to_ground_clause (P \<cdot> \<gamma>') \<and> term_subst.is_ground_subst \<gamma>'
-              \<and> welltyped\<^sub>c typeof_fun \<V> P \<and> (\<exists>\<F>\<^sub>G. welltyped\<^sub>\<sigma> \<F>\<^sub>G \<V> \<gamma>' \<and> typeof_fun \<subseteq>\<^sub>m \<F>\<^sub>G)) 
+              \<and> welltyped\<^sub>c typeof_fun \<V> P \<and> welltyped\<^sub>\<sigma> typeof_fun \<V> \<gamma>') 
             \<longrightarrow> upair ` I \<TTurnstile> P\<^sub>G; 
        term_subst.is_ground_subst \<gamma>;
-       welltyped\<^sub>c typeof_fun \<V> C; welltyped\<^sub>\<sigma> \<F>\<^sub>G \<V> \<gamma>; typeof_fun \<subseteq>\<^sub>m \<F>\<^sub>G
+       welltyped\<^sub>c typeof_fun \<V> C; welltyped\<^sub>\<sigma> typeof_fun \<V> \<gamma>
      \<rbrakk> \<Longrightarrow> upair  ` I \<TTurnstile> to_ground_clause (C \<cdot> \<gamma>)"
    proof-
-    fix I :: "'f gterm rel" and \<gamma> :: "('f, 'v) subst" and \<F>\<^sub>G
+    fix I :: "'f gterm rel" and \<gamma> :: "('f, 'v) subst"
     
     let ?I = "upair ` I"
     
@@ -37,9 +37,9 @@ proof (cases P C rule: eq_resolution.cases)
      refl_I: "refl I" and 
      premise: 
       "\<forall>P\<^sub>G. (\<exists>\<gamma>'. P\<^sub>G = to_ground_clause (P \<cdot> \<gamma>') \<and> term_subst.is_ground_subst \<gamma>'
-             \<and> welltyped\<^sub>c typeof_fun \<V> P \<and> (\<exists>\<F>\<^sub>G. welltyped\<^sub>\<sigma> \<F>\<^sub>G \<V> \<gamma>' \<and> typeof_fun \<subseteq>\<^sub>m \<F>\<^sub>G)) \<longrightarrow> ?I \<TTurnstile> P\<^sub>G" and
+             \<and> welltyped\<^sub>c typeof_fun \<V> P \<and> welltyped\<^sub>\<sigma> typeof_fun \<V> \<gamma>') \<longrightarrow> ?I \<TTurnstile> P\<^sub>G" and
      grounding: "term_subst.is_ground_subst \<gamma>" and
-     wt: "welltyped\<^sub>c typeof_fun \<V> C" "welltyped\<^sub>\<sigma> \<F>\<^sub>G \<V> \<gamma>" "typeof_fun \<subseteq>\<^sub>m \<F>\<^sub>G"
+     wt: "welltyped\<^sub>c typeof_fun \<V> C" "welltyped\<^sub>\<sigma> typeof_fun \<V> \<gamma>"
 
     let ?P = "to_ground_clause (P \<cdot> \<mu> \<cdot> \<gamma>)"
     let ?L = "to_ground_literal (L \<cdot>l \<mu> \<cdot>l \<gamma>)"
@@ -52,23 +52,23 @@ proof (cases P C rule: eq_resolution.cases)
       by blast
 
     moreover have welltyped_\<mu>: "welltyped\<^sub>\<sigma> typeof_fun \<V> \<mu>"
-      using eq_resolutionI(6)
+      using eq_resolutionI(6) wt(1)
       by auto
 
     ultimately have welltyped_P': "welltyped\<^sub>c typeof_fun \<V> P'"
       using welltyped\<^sub>\<sigma>_welltyped\<^sub>c
       by blast
 
-    from welltyped_\<mu> have "welltyped\<^sub>\<sigma> \<F>\<^sub>G \<V> (\<mu> \<odot> \<gamma>)"
-      using wt(2) welltyped\<^sub>\<sigma>_map_le[OF welltyped_\<mu> wt(3)]
+    from welltyped_\<mu> have "welltyped\<^sub>\<sigma> typeof_fun \<V> (\<mu> \<odot> \<gamma>)"
+      using wt(2)
       by (simp add: subst_compose_def welltyped\<^sub>\<sigma>_def welltyped\<^sub>\<sigma>_welltyped)
 
     moreover have "welltyped\<^sub>c typeof_fun \<V> (add_mset (s\<^sub>1 !\<approx> s\<^sub>2) P')"
-      using eq_resolutionI(6) welltyped_add_literal[OF welltyped_P']
+      using eq_resolutionI(6) welltyped_add_literal[OF welltyped_P'] wt(1)
       by auto
 
     ultimately have "?I \<TTurnstile> ?P"
-      using premise[rule_format, of ?P, OF exI, of "\<mu> \<odot> \<gamma>"] wt(1,3) grounding ground_subst_compose
+      using premise[rule_format, of ?P, OF exI, of "\<mu> \<odot> \<gamma>"] grounding ground_subst_compose
       using eq_resolutionI
       by auto
 
@@ -115,7 +115,8 @@ proof (cases P C rule: eq_resolution.cases)
    qed
     
    then show ?thesis
-      unfolding ground.G_entails_def true_clss_def clause_groundings_def
+     unfolding ground.G_entails_def true_clss_def clause_groundings_def
+     apply auto
      using eq_resolutionI(1, 2) by auto
 qed
 
@@ -131,13 +132,13 @@ proof (cases P C rule: eq_factoring.cases)
         trans I; 
         sym I;
         \<forall>P\<^sub>G. (\<exists>\<gamma>'. P\<^sub>G = to_ground_clause (P \<cdot> \<gamma>') \<and> term_subst.is_ground_subst \<gamma>'
-              \<and> welltyped\<^sub>c typeof_fun \<V> P \<and> (\<exists>\<F>\<^sub>G. welltyped\<^sub>\<sigma> \<F>\<^sub>G \<V> \<gamma>' \<and> typeof_fun \<subseteq>\<^sub>m \<F>\<^sub>G)) 
+              \<and> welltyped\<^sub>c typeof_fun \<V> P \<and> welltyped\<^sub>\<sigma> typeof_fun \<V> \<gamma>') 
             \<longrightarrow> upair ` I \<TTurnstile> P\<^sub>G; 
        term_subst.is_ground_subst \<gamma>;
-       welltyped\<^sub>c typeof_fun \<V> C; welltyped\<^sub>\<sigma> \<F>\<^sub>G \<V> \<gamma>; typeof_fun \<subseteq>\<^sub>m \<F>\<^sub>G
+       welltyped\<^sub>c typeof_fun \<V> C; welltyped\<^sub>\<sigma> typeof_fun \<V> \<gamma>
      \<rbrakk> \<Longrightarrow> upair  ` I \<TTurnstile> to_ground_clause (C \<cdot> \<gamma>)"
   proof-
-    fix I :: "'f gterm rel" and \<gamma> :: "'v \<Rightarrow> ('f, 'v) Term.term" and \<F>\<^sub>G
+    fix I :: "'f gterm rel" and \<gamma> :: "'v \<Rightarrow> ('f, 'v) Term.term"
 
     let ?I = "upair ` I"
     
@@ -146,9 +147,9 @@ proof (cases P C rule: eq_factoring.cases)
      sym_I: "sym I" and 
      premise: 
        "\<forall>P\<^sub>G. (\<exists>\<gamma>'. P\<^sub>G = to_ground_clause (P \<cdot> \<gamma>') \<and> term_subst.is_ground_subst \<gamma>'
-             \<and> welltyped\<^sub>c typeof_fun \<V> P \<and> (\<exists>\<F>\<^sub>G. welltyped\<^sub>\<sigma> \<F>\<^sub>G \<V> \<gamma>' \<and> typeof_fun \<subseteq>\<^sub>m \<F>\<^sub>G)) \<longrightarrow> ?I \<TTurnstile> P\<^sub>G" and
+             \<and> welltyped\<^sub>c typeof_fun \<V> P \<and> welltyped\<^sub>\<sigma> typeof_fun \<V> \<gamma>') \<longrightarrow> ?I \<TTurnstile> P\<^sub>G" and
      grounding: "term_subst.is_ground_subst \<gamma>" and
-     wt: "welltyped\<^sub>c typeof_fun \<V> C" "welltyped\<^sub>\<sigma> \<F>\<^sub>G \<V> \<gamma>" "typeof_fun \<subseteq>\<^sub>m \<F>\<^sub>G"
+     wt: "welltyped\<^sub>c typeof_fun \<V> C" "welltyped\<^sub>\<sigma> typeof_fun \<V> \<gamma>"
 
     let ?P = "to_ground_clause (P \<cdot> \<mu> \<cdot> \<gamma>)"
     let ?P' = "to_ground_clause (P' \<cdot> \<mu> \<cdot> \<gamma>)"
@@ -169,7 +170,7 @@ proof (cases P C rule: eq_factoring.cases)
       by auto
       
     moreover have welltyped_\<mu>: "welltyped\<^sub>\<sigma> typeof_fun \<V> \<mu>"
-      using eq_factoringI(10)
+      using eq_factoringI(10) wt(1)
       by blast
 
     ultimately have welltyped_P': "welltyped\<^sub>c typeof_fun \<V> P'"
@@ -186,12 +187,12 @@ proof (cases P C rule: eq_factoring.cases)
       by (smt (verit, best) insert_iff set_uprod_simps upair_in_literal(1) upair_in_literal(2))
 
     have welltyped_L\<^sub>2: "welltyped\<^sub>l typeof_fun \<V> (t\<^sub>2 \<approx> t\<^sub>2')"
-      using xx right_uniqueD[OF welltyped_right_unique] eq_factoringI(10)
+      using xx right_uniqueD[OF welltyped_right_unique] eq_factoringI(10) wt(1)
       unfolding welltyped\<^sub>l_def welltyped\<^sub>a_def
       by (smt (verit) insert_iff set_uprod_simps upair_in_literal(1))
 
-    from welltyped_\<mu> have "welltyped\<^sub>\<sigma> \<F>\<^sub>G \<V> (\<mu> \<odot> \<gamma>)"
-      using wt(2) welltyped\<^sub>\<sigma>_map_le[OF welltyped_\<mu> wt(3)]
+    from welltyped_\<mu> have "welltyped\<^sub>\<sigma> typeof_fun \<V> (\<mu> \<odot> \<gamma>)"
+      using wt(2) 
       by (simp add: subst_compose_def welltyped\<^sub>\<sigma>_def welltyped\<^sub>\<sigma>_welltyped)
 
     moreover have "welltyped\<^sub>c typeof_fun \<V> P"
@@ -202,7 +203,6 @@ proof (cases P C rule: eq_factoring.cases)
     ultimately have "?I \<TTurnstile> ?P"
       using 
         premise[rule_format, of ?P, OF exI, of "\<mu> \<odot> \<gamma>"] 
-        wt(1,3) 
         ground_subst_compose grounding
       by auto
       
@@ -268,7 +268,7 @@ lemma superposition_sound:
   shows "{P1, P2} \<TTurnstile>\<^sub>F {C}"
   using step
 proof (cases P2 P1 C rule: superposition.cases)
-  case (superpositionI \<rho>\<^sub>1 \<rho>\<^sub>2 L\<^sub>1 P\<^sub>1' L\<^sub>2 P\<^sub>2' \<P> s\<^sub>1 u\<^sub>1 s\<^sub>1' t\<^sub>2 t\<^sub>2' \<mu>)
+  case (superpositionI \<rho>\<^sub>1 \<rho>\<^sub>2 P\<^sub>1 P\<^sub>2 L\<^sub>1 P\<^sub>1' L\<^sub>2 P\<^sub>2' \<P> s\<^sub>1 u\<^sub>1 s\<^sub>1' t\<^sub>2 t\<^sub>2' \<mu> \<V>\<^sub>3 \<V>\<^sub>1 \<V>\<^sub>2 C)
 
   have 
     "\<And>I \<gamma>. \<lbrakk>
@@ -276,9 +276,9 @@ proof (cases P2 P1 C rule: superposition.cases)
         trans I; 
         sym I;
         compatible_with_gctxt I;
-        \<forall>P\<^sub>G. (\<exists>\<gamma>'. P\<^sub>G = to_ground_clause (P1 \<cdot> \<gamma>') \<and> is_ground_clause (P1 \<cdot> \<gamma>')) \<longrightarrow> upair ` I \<TTurnstile> P\<^sub>G;
-        \<forall>P\<^sub>G. (\<exists>\<gamma>'. P\<^sub>G = to_ground_clause (P2 \<cdot> \<gamma>') \<and> is_ground_clause (P2 \<cdot> \<gamma>')) \<longrightarrow> upair ` I \<TTurnstile> P\<^sub>G;
-        is_ground_clause (C \<cdot> \<gamma>)
+        \<forall>P\<^sub>G. (\<exists>\<gamma>'. P\<^sub>G = to_ground_clause (P\<^sub>1 \<cdot> \<gamma>') \<and> term_subst.is_ground_subst \<gamma>' \<and> welltyped\<^sub>c typeof_fun \<V>\<^sub>1 P\<^sub>1 \<and> welltyped\<^sub>\<sigma> typeof_fun \<V>\<^sub>1 \<gamma>') \<longrightarrow> upair ` I \<TTurnstile> P\<^sub>G;
+        \<forall>P\<^sub>G. (\<exists>\<gamma>'. P\<^sub>G = to_ground_clause (P\<^sub>2 \<cdot> \<gamma>') \<and> term_subst.is_ground_subst \<gamma>' \<and> welltyped\<^sub>c typeof_fun \<V>\<^sub>2 P\<^sub>2 \<and> welltyped\<^sub>\<sigma> typeof_fun \<V>\<^sub>2 \<gamma>') \<longrightarrow> upair ` I \<TTurnstile> P\<^sub>G;
+        term_subst.is_ground_subst \<gamma>; welltyped\<^sub>c typeof_fun \<V>\<^sub>3 C; welltyped\<^sub>\<sigma> typeof_fun \<V>\<^sub>3 \<gamma>
      \<rbrakk> \<Longrightarrow> (\<lambda>(x, y). Upair x y) ` I \<TTurnstile> to_ground_clause (C \<cdot> \<gamma>)"
   proof -
     fix I :: "'f gterm rel" and \<gamma> :: "'v \<Rightarrow> ('f, 'v) Term.term"
@@ -291,71 +291,97 @@ proof (cases P2 P1 C rule: superposition.cases)
       sym_I: "sym I" and 
       compatible_with_ground_context_I: "compatible_with_gctxt I" and
       premise1: 
-        "\<forall>P\<^sub>G. (\<exists>\<gamma>'. P\<^sub>G = to_ground_clause (P1 \<cdot> \<gamma>') \<and> is_ground_clause (P1 \<cdot> \<gamma>')) \<longrightarrow>?I \<TTurnstile> P\<^sub>G" and
+        "\<forall>P\<^sub>G. (\<exists>\<gamma>'. P\<^sub>G = to_ground_clause (P\<^sub>1 \<cdot> \<gamma>') \<and> term_subst.is_ground_subst \<gamma>' \<and> welltyped\<^sub>c typeof_fun \<V>\<^sub>1 P\<^sub>1 \<and> welltyped\<^sub>\<sigma> typeof_fun \<V>\<^sub>1 \<gamma>') \<longrightarrow>?I \<TTurnstile> P\<^sub>G" and
       premise2: 
-        "\<forall>P\<^sub>G. (\<exists>\<gamma>'. P\<^sub>G = to_ground_clause (P2 \<cdot> \<gamma>') \<and> is_ground_clause (P2 \<cdot> \<gamma>')) \<longrightarrow> ?I \<TTurnstile> P\<^sub>G" and 
-      conclusion_grounding: "is_ground_clause (C \<cdot> \<gamma>)"
-
-     obtain \<gamma>' :: "'v \<Rightarrow> ('f, 'v) Term.term" where 
-       \<gamma>': "term_subst.is_ground_subst \<gamma>'" "C \<cdot> \<gamma> = C \<cdot> \<gamma>'"
-       using ground_subst_exstension_clause[OF conclusion_grounding]
-       by blast
+        "\<forall>P\<^sub>G. (\<exists>\<gamma>'. P\<^sub>G = to_ground_clause (P\<^sub>2 \<cdot> \<gamma>') \<and> term_subst.is_ground_subst \<gamma>' \<and> welltyped\<^sub>c typeof_fun \<V>\<^sub>2 P\<^sub>2 \<and> welltyped\<^sub>\<sigma> typeof_fun \<V>\<^sub>2 \<gamma>') \<longrightarrow> ?I \<TTurnstile> P\<^sub>G" and 
+      grounding: "term_subst.is_ground_subst \<gamma>" "welltyped\<^sub>c typeof_fun \<V>\<^sub>3 C" "welltyped\<^sub>\<sigma> typeof_fun \<V>\<^sub>3 \<gamma>"
       
-     let ?P1 = "to_ground_clause (P1 \<cdot> \<rho>\<^sub>1 \<cdot> \<mu> \<cdot> \<gamma>')"
-     let ?P2 = "to_ground_clause (P2 \<cdot> \<rho>\<^sub>2 \<cdot> \<mu> \<cdot> \<gamma>')"
+     let ?P\<^sub>1 = "to_ground_clause (P\<^sub>1 \<cdot> \<rho>\<^sub>1 \<cdot> \<mu> \<cdot> \<gamma>)"
+     let ?P\<^sub>2 = "to_ground_clause (P\<^sub>2 \<cdot> \<rho>\<^sub>2 \<cdot> \<mu> \<cdot> \<gamma>)"
   
-     let ?L\<^sub>1 = "to_ground_literal (L\<^sub>1 \<cdot>l \<rho>\<^sub>1 \<cdot>l \<mu> \<cdot>l \<gamma>')"
-     let ?L\<^sub>2 = "to_ground_literal (L\<^sub>2 \<cdot>l \<rho>\<^sub>2 \<cdot>l \<mu> \<cdot>l \<gamma>')"
+     let ?L\<^sub>1 = "to_ground_literal (L\<^sub>1 \<cdot>l \<rho>\<^sub>1 \<cdot>l \<mu> \<cdot>l \<gamma>)"
+     let ?L\<^sub>2 = "to_ground_literal (L\<^sub>2 \<cdot>l \<rho>\<^sub>2 \<cdot>l \<mu> \<cdot>l \<gamma>)"
   
-     let ?P\<^sub>1' = "to_ground_clause (P\<^sub>1' \<cdot> \<rho>\<^sub>1 \<cdot> \<mu> \<cdot> \<gamma>')"
-     let ?P\<^sub>2' = "to_ground_clause (P\<^sub>2' \<cdot> \<rho>\<^sub>2 \<cdot> \<mu> \<cdot> \<gamma>')"
+     let ?P\<^sub>1' = "to_ground_clause (P\<^sub>1' \<cdot> \<rho>\<^sub>1 \<cdot> \<mu> \<cdot> \<gamma>)"
+     let ?P\<^sub>2' = "to_ground_clause (P\<^sub>2' \<cdot> \<rho>\<^sub>2 \<cdot> \<mu> \<cdot> \<gamma>)"
   
-     let ?s\<^sub>1 = "to_ground_context (s\<^sub>1 \<cdot>t\<^sub>c \<rho>\<^sub>1 \<cdot>t\<^sub>c \<mu> \<cdot>t\<^sub>c \<gamma>')"
-     let ?s\<^sub>1' = "to_ground_term (s\<^sub>1' \<cdot>t \<rho>\<^sub>1 \<cdot>t \<mu> \<cdot>t \<gamma>')"
-     let ?t\<^sub>2 = "to_ground_term (t\<^sub>2 \<cdot>t \<rho>\<^sub>2 \<cdot>t \<mu> \<cdot>t \<gamma>')"
-     let ?t\<^sub>2' = "to_ground_term (t\<^sub>2' \<cdot>t \<rho>\<^sub>2 \<cdot>t \<mu> \<cdot>t \<gamma>')"
-     let ?u\<^sub>1 = "to_ground_term (u\<^sub>1 \<cdot>t \<rho>\<^sub>1 \<cdot>t \<mu> \<cdot>t \<gamma>')"
+     let ?s\<^sub>1 = "to_ground_context (s\<^sub>1 \<cdot>t\<^sub>c \<rho>\<^sub>1 \<cdot>t\<^sub>c \<mu> \<cdot>t\<^sub>c \<gamma>)"
+     let ?s\<^sub>1' = "to_ground_term (s\<^sub>1' \<cdot>t \<rho>\<^sub>1 \<cdot>t \<mu> \<cdot>t \<gamma>)"
+     let ?t\<^sub>2 = "to_ground_term (t\<^sub>2 \<cdot>t \<rho>\<^sub>2 \<cdot>t \<mu> \<cdot>t \<gamma>)"
+     let ?t\<^sub>2' = "to_ground_term (t\<^sub>2' \<cdot>t \<rho>\<^sub>2 \<cdot>t \<mu> \<cdot>t \<gamma>)"
+     let ?u\<^sub>1 = "to_ground_term (u\<^sub>1 \<cdot>t \<rho>\<^sub>1 \<cdot>t \<mu> \<cdot>t \<gamma>)"
   
      let ?\<P> = "if \<P> = Pos then Pos else Neg"
   
-     let ?C = "to_ground_clause (C \<cdot> \<gamma>')"
+     let ?C = "to_ground_clause (C \<cdot> \<gamma>)"
 
-     have "?I \<TTurnstile> ?P1"
-       using premise1[rule_format, of ?P1, OF exI, of "\<rho>\<^sub>1 \<odot> \<mu> \<odot> \<gamma>'"] \<gamma>'
-       by (simp add: is_ground_subst_is_ground_clause)
+     have ground_subst: 
+       "term_subst.is_ground_subst (\<rho>\<^sub>1 \<odot> \<mu> \<odot> \<gamma>)" 
+       "term_subst.is_ground_subst (\<rho>\<^sub>2 \<odot> \<mu> \<odot> \<gamma>)"
+       using ground_subst_compose[OF grounding(1)]
+       by blast+
 
-     moreover have "?I \<TTurnstile> ?P2"
-       using premise2[rule_format, of ?P2, OF exI, of "\<rho>\<^sub>2 \<odot> \<mu> \<odot> \<gamma>'"] \<gamma>'
-       by (simp add: is_ground_subst_is_ground_clause)
+     have wt_P: "welltyped\<^sub>c typeof_fun \<V>\<^sub>1 P\<^sub>1" "welltyped\<^sub>c typeof_fun \<V>\<^sub>2 P\<^sub>2"
+       using grounding(2) superpositionI(9)
+       unfolding superpositionI welltyped\<^sub>c_def welltyped\<^sub>l_def welltyped\<^sub>a_def subst_clause_add_mset
+        apply auto
+       unfolding subst_literal subst_atom
+       apply auto
+       sorry
+
+     have 
+       "\<And>\<sigma>. welltyped\<^sub>\<sigma> typeof_fun \<V>\<^sub>3 \<sigma> \<Longrightarrow> welltyped\<^sub>\<sigma> typeof_fun \<V>\<^sub>1 (\<rho>\<^sub>1 \<odot> \<sigma>)"
+       "\<And>\<sigma>. welltyped\<^sub>\<sigma> typeof_fun \<V>\<^sub>3 \<sigma> \<Longrightarrow> welltyped\<^sub>\<sigma> typeof_fun \<V>\<^sub>2 (\<rho>\<^sub>2 \<odot> \<sigma>)"
+       using superpositionI(15-18) superpositionI(4-5)
+       unfolding welltyped\<^sub>\<sigma>_def
+      
+       sorry
+
+     then have wt_\<gamma>: "welltyped\<^sub>\<sigma> typeof_fun \<V>\<^sub>1 (\<rho>\<^sub>1 \<odot> \<mu> \<odot> \<gamma>)" "welltyped\<^sub>\<sigma> typeof_fun \<V>\<^sub>2 (\<rho>\<^sub>2 \<odot> \<mu> \<odot> \<gamma>)"
+       using superpositionI(14-18) 
+       unfolding welltyped\<^sub>\<sigma>_def
+       by (metis (no_types, lifting) grounding(3) subst_compose_assoc subst_compose_def welltyped\<^sub>\<sigma>_welltyped)+
+
+     have "?I \<TTurnstile> ?P\<^sub>1"
+       using premise1[rule_format, of ?P\<^sub>1, OF exI, of "\<rho>\<^sub>1 \<odot> \<mu> \<odot> \<gamma>"] ground_subst wt_P  wt_\<gamma>
+       by auto
+
+     moreover have "?I \<TTurnstile> ?P\<^sub>2"
+       using premise2[rule_format, of ?P\<^sub>2, OF exI, of "\<rho>\<^sub>2 \<odot> \<mu> \<odot> \<gamma>"]  ground_subst wt_P  wt_\<gamma>
+       by auto
 
      ultimately obtain L\<^sub>1' L\<^sub>2' 
        where
-         L\<^sub>1'_in_P1: "L\<^sub>1' \<in># ?P1" and 
+         L\<^sub>1'_in_P1: "L\<^sub>1' \<in># ?P\<^sub>1" and 
          I_models_L\<^sub>1': "?I \<TTurnstile>l L\<^sub>1'" and
-         L\<^sub>2'_in_P2: "L\<^sub>2' \<in># ?P2" and 
+         L\<^sub>2'_in_P2: "L\<^sub>2' \<in># ?P\<^sub>2" and 
          I_models_L\<^sub>2': "?I \<TTurnstile>l L\<^sub>2'"
        by (auto simp: true_cls_def)
 
      have u\<^sub>1_equals_t\<^sub>2: "?t\<^sub>2 = ?u\<^sub>1"
-       using term_subst.subst_imgu_eq_subst_imgu[OF superpositionI(10)]
-       by simp
+       using term_subst.subst_imgu_eq_subst_imgu[OF superpositionI(13)]
+       by argo
 
-     have s\<^sub>1_u\<^sub>1: "?s\<^sub>1\<langle>?u\<^sub>1\<rangle>\<^sub>G = to_ground_term (s\<^sub>1 \<cdot>t\<^sub>c \<rho>\<^sub>1 \<cdot>t\<^sub>c \<mu> \<cdot>t\<^sub>c \<gamma>')\<langle>u\<^sub>1 \<cdot>t \<rho>\<^sub>1 \<cdot>t \<mu> \<cdot>t \<gamma>'\<rangle>"
-       using ground_term_with_context(1)[OF 
-              is_ground_subst_is_ground_context[OF \<gamma>'(1)] 
-              is_ground_subst_is_ground_term[OF \<gamma>'(1)]
-            ]
+     have s\<^sub>1_u\<^sub>1: "?s\<^sub>1\<langle>?u\<^sub>1\<rangle>\<^sub>G = to_ground_term (s\<^sub>1 \<cdot>t\<^sub>c \<rho>\<^sub>1 \<cdot>t\<^sub>c \<mu> \<cdot>t\<^sub>c \<gamma>)\<langle>u\<^sub>1 \<cdot>t \<rho>\<^sub>1 \<cdot>t \<mu> \<cdot>t \<gamma>\<rangle>"
+       using 
+         ground_term_with_context(1)[OF 
+            is_ground_subst_is_ground_context
+            is_ground_subst_is_ground_term
+          ]
+         grounding(1) 
        by blast
 
-    have s\<^sub>1_t\<^sub>2': "(?s\<^sub>1)\<langle>?t\<^sub>2'\<rangle>\<^sub>G  = to_ground_term (s\<^sub>1 \<cdot>t\<^sub>c \<rho>\<^sub>1 \<cdot>t\<^sub>c \<mu> \<cdot>t\<^sub>c \<gamma>')\<langle>t\<^sub>2' \<cdot>t \<rho>\<^sub>2 \<cdot>t \<mu> \<cdot>t \<gamma>'\<rangle>"
-      using ground_term_with_context(1)[OF 
-              is_ground_subst_is_ground_context[OF \<gamma>'(1)] 
-              is_ground_subst_is_ground_term[OF \<gamma>'(1)]
-            ]
+    have s\<^sub>1_t\<^sub>2': "(?s\<^sub>1)\<langle>?t\<^sub>2'\<rangle>\<^sub>G  = to_ground_term (s\<^sub>1 \<cdot>t\<^sub>c \<rho>\<^sub>1 \<cdot>t\<^sub>c \<mu> \<cdot>t\<^sub>c \<gamma>)\<langle>t\<^sub>2' \<cdot>t \<rho>\<^sub>2 \<cdot>t \<mu> \<cdot>t \<gamma>\<rangle>"
+      using 
+        ground_term_with_context(1)[OF 
+          is_ground_subst_is_ground_context
+          is_ground_subst_is_ground_term
+        ]
+        grounding(1)
       by blast
       
     have \<P>_pos_or_neg: "\<P> = Pos \<or> \<P> = Neg"
-      using superpositionI(6) by blast
+      using superpositionI(9) by blast
 
     then have L\<^sub>1: "?L\<^sub>1 = ?\<P> (Upair ?s\<^sub>1\<langle>?u\<^sub>1\<rangle>\<^sub>G ?s\<^sub>1')"
       unfolding superpositionI to_ground_literal_def to_ground_atom_def
@@ -386,7 +412,7 @@ proof (cases P2 P1 C rule: superposition.cases)
         case L\<^sub>2'_def: True
 
         then have ts_in_I: "(?t\<^sub>2, ?t\<^sub>2') \<in> I"
-          using I_models_L\<^sub>2' true_lit_uprod_iff_true_lit_prod[OF sym_I] superpositionI(8)
+          using I_models_L\<^sub>2' true_lit_uprod_iff_true_lit_prod[OF sym_I] superpositionI(11)
           unfolding to_ground_literal_def to_ground_atom_def 
           by (smt (verit) literal.simps(9) map_uprod_simps subst_atom_def subst_literal true_lit_simps(1)) 
 
@@ -405,7 +431,7 @@ proof (cases P2 P1 C rule: superposition.cases)
             by blast
 
           then show ?thesis 
-            unfolding C that \<gamma>'
+            unfolding C that
             by (smt (verit) true_cls_add_mset)
         qed
 
@@ -424,7 +450,7 @@ proof (cases P2 P1 C rule: superposition.cases)
             by (meson true_lit_uprod_iff_true_lit_prod(2) sym_I true_lit_simps(2))
 
           then show ?thesis 
-            unfolding C that \<gamma>'
+            unfolding C that
             by (smt (verit, best) literals_distinct(1) true_cls_add_mset)
         qed
 
@@ -442,7 +468,7 @@ proof (cases P2 P1 C rule: superposition.cases)
 
         then show ?thesis
           unfolding superpositionI 
-          by (metis C \<gamma>'(2) local.superpositionI(19) true_cls_union union_mset_add_mset_left)
+          by (metis C local.superpositionI(25) true_cls_union union_mset_add_mset_left)
       qed
     next
       case False
@@ -455,14 +481,13 @@ proof (cases P2 P1 C rule: superposition.cases)
         using I_models_L\<^sub>1' by blast
 
       then show ?thesis 
-        unfolding \<gamma>'(2)
         unfolding superpositionI
         by (simp add: to_ground_clause_def subst_clause_add_mset subst_clause_plus)
     qed
   qed
 
   then show ?thesis 
-    unfolding ground.G_entails_def clause_groundings_def true_clss_def
+    unfolding ground.G_entails_def clause_groundings_def true_clss_def superpositionI(1-3)
     by auto
 qed
 
@@ -492,7 +517,7 @@ proof-
     where select\<^sub>G = select\<^sub>G
     by unfold_locales (simp add: select\<^sub>G\<^sub>s_def)
 
-  show "sound_inference_system inferences {{#}} entails_\<G>"
+  show "sound_inference_system inferences \<bottom>\<^sub>F entails_\<G>"
     using sound_inference_system_axioms Q_nonempty[folded ex_in_conv]
     unfolding entails_def
     by simp
